---
topics:
    - Fourier analysis
---

<problem>

Given $f \in L^2\p{\br{0,\pi}}$, we say that $f \in \mathcal{G}$ if $f$ admits a representation of the form

$$
f\p{x} = \sum_{n=0}^\infty c_n\cos{nx}
\quad\text{with}\quad \sum_{n=0}^\infty \p{1 + n^2}\abs{c_n}^2 < \infty.
$$

Show that if $f \in \mathcal{G}$ and $g \in \mathcal{G}$, then $fg \in \mathcal{G}$.

</problem>

<solution>

Write $f\p{x} = \sum_{n=0}^\infty c_n\cos{nx}$ and $g\p{x} = \sum_{n=0}^\infty d_n\cos{nx}$ with the convergence properties given. Observe that

$$
\begin{aligned}
    f\p{x}g\p{x}
        &= \sum_{n=0}^\infty \sum_{m=0}^\infty c_nd_m \cos{nx} \cos{mx} \\
        &= \sum_{n=0}^\infty \sum_{m=0}^\infty \frac{c_nd_m}{2} \p{\cos{\p{n + m}x} + \cos{\p{n - m}x}} \\
        &\eqqcolon \sum_{k=0}^\infty a_k\cos{kx},
\end{aligned}
$$

so $fg$ can be represented in the right form as long as the sum converges absolutely (and hence may be rearranged). This is indeed the case, as

$$
\begin{aligned}
    \sum_{n=0}^\infty \sum_{m=0}^\infty \abs{c_nd_m \cos{nx} \cos{mx}}
        &\leq \p{\sum_{n=0}^\infty \abs{c_n}} \p{\sum_{m=0}^\infty \abs{d_m}} \\
        &= \p{\sum_{n=0}^\infty \sqrt{1 + n^2}\abs{c_n} \cdot \frac{1}{\sqrt{1 + n^2}}} \p{\sum_{m=0}^\infty \sqrt{1 + m^2}\abs{d_m} \cdot \frac{1}{\sqrt{1 + m^2}}} \\
        &\leq \p{\sum_{n=0}^\infty \p{1 + n^2}\abs{c_n}^2}^{1/2} \p{\sum_{m=0}^\infty \p{1 + m^2}\abs{d_m}^2}^{1/2} \sum_{n=0}^\infty \frac{1}{1 + n^2} \\
        &< \infty,
\end{aligned}
$$

so the sum converges absolutely. By absolute convergence and orthogonality, we get

$$
\begin{aligned}
    \int_0^\pi \abs{f\p{x}g\p{x}}^2 \,\diff{x}
        &= \int_0^\pi \abs{\p{\sum_{k=0}^\infty a_k\cos{kx}} \p{\sum_{\ell=0}^\infty a_\ell\cos{\ell x}}} \,\diff{x} \\
        &\leq \sum_{k=0}^\infty \int_0^\pi \abs{a_k}^2 \cos^2{kx} \,\diff{x} \\
        &= \frac{\pi}{2} \sum_{k=0}^\infty \abs{a_k}^2.
\end{aligned}
$$

Hence, if we show that $\sum_{k=0}^\infty \p{1 + k^2}\abs{a_k}^2 < \infty$, then we will have shown that $fg \in L^2$ as well. Since we are working with non-negative values, we may re-order the terms:

$$
\begin{aligned}
    \sum_{k=0}^\infty \p{1 + k^2}\abs{a_k}^2
        &= \frac{1}{4} \sum_{n=0}^\infty \sum_{m=0}^\infty \abs{c_nd_m}^2\p{\p{1 + \p{n + m}^2} + \p{1 + \p{n - m}^2}} \\
        &= \frac{1}{2} \sum_{n=0}^\infty \sum_{m=0}^\infty \abs{c_nd_m}^2 \p{1 + m^2 + n^2} \\
        &\leq \frac{1}{2} \sum_{n=0}^\infty \sum_{m=0}^\infty \abs{c_nd_m}^2 \p{1 + m^2}\p{1 + n^2} \\
        &= \frac{1}{2} \p{\sum_{n=0}^\infty \p{1 + n^2}\abs{c_n}^2} \p{\sum_{m=0}^\infty \p{1 + m^2}\abs{d_m}^2} \\
        &< \infty,
\end{aligned}
$$

so $fg \in \mathcal{G}$.

</solution>
