---
topics:
    - measure theory
---

<problem>

Suppose $\func{f}{\R}{\R}$ is a bounded and measurable function satisfying $f\p{x + 1} = f\p{x}$ and $f\p{2x} = f\p{x}$ for almost every $x \in \R$. Show that then there exists a constant $c \in \R$ such that $f\p{x} = c$ for almost every $x \in \R$.

</problem>

<solution>

First, observe that on any dyadic interval $\br{\frac{k}{2^n}, \frac{k+1}{2^n}} \subseteq \br{0, 1}$, i.e., $0 \leq k \leq 2^n - 1$ and $n \geq 0$, we have

$$
\int_{k/2^n}^{\p{k+1}/2^n} f \,\diff{x}
    = \frac{1}{2^n} \int_k^{k+1} f \,\diff{x}
    = \frac{1}{2^n} \int_0^1 f \,\diff{x}.
$$

Let $c = \int_0^1 f \,\diff{x}$ and consider $f_n = 2^{n} \int_{k/2^n}^{\p{k+1}/2^n} f \,\diff{x}$ on $\br{\frac{k}{2^n}, \frac{k+1}{2^n}}$ and $0$ otherwise. If we show that $f_n \to f$ in $L^1\p{\br{0, 1}}$, then

$$
\norm{f_n - f}_{L^1\p{\br{0,1}}}
    = \int_0^1 \abs{f_n - f} \,\diff{x}
    = \int_0^1 \abs{c - f} \,\diff{x} \xrightarrow{n\to\infty} 0,
$$

so $\int_0^1 \abs{c - f} \,\diff{x} = 0$ and so $f = c$ for almost every $x \in \br{0, 1}$. Thus, by the translation invariance of $f$ almost everywhere,

$$
\int_k^{k+1} \abs{f - c} \,\diff{x}
    = \int_0^1 \abs{f - c} \,\diff{x}
    = 0,
$$

so $f = c$ for almost every $x \in \R$. Hence, it remains to prove the $L^1$ convergence.

Let $A_{k,n}\p{g} = \int_{k/2^n}^{\p{k+1}/2^n} \abs{g} \,\diff{x}$. First, note that

$$
A_{k,n}\p{1}
    = 2^n \int_{k/2^n}^{\p{k+1}/2^n} \,\diff{x}
    = 1.
$$

Let $\epsilon > 0$ and let $g$ be a continuous function on $\br{0, 1}$ such that $\norm{f - g}_{L^1} < \epsilon$. Then

$$
\begin{aligned}
    \norm{f_n - f}_{L^1\p{\br{0,1}}}
        &= \int_0^1 \abs{f_n - f} \,\diff{x} \\
        &= \sum_{k=0}^{2^n-1} \int_{k/2^n}^{\p{k+1}/2^n} \abs{2^n  \int_{k/2^n}^{\p{k+1}/2^n} f\p{y} - f\p{x} \,\diff{y}} \,\diff{x} \\
        &\leq \sum_{k=0}^{2^n-1} \int_{k/2^n}^{\p{k+1}/2^n} 2^n  \int_{k/2^n}^{\p{k+1}/2^n} \abs{f\p{y} - f\p{x}} \,\diff{y} \,\diff{x} \\
        &\leq \sum_{k=0}^{2^n-1} \int_{k/2^n}^{\p{k+1}/2^n} A_{k,n}\p{f - g} + A_{k,n}\p{f\p{x} - g\p{x}} + A_{k,n}\p{g - g\p{x}} \,\diff{x}.
\end{aligned}
$$

We estimate separately:

$$
\begin{aligned}
    \int_{k/2^n}^{\p{k+1}/2^n} A_{k,n}\p{f - g} \,\diff{x}
        &= \int_{k/2^n}^{\p{k+1}/2^n} 2^n \int_{k/2^n}^{\p{k+1}/2^n} \abs{f\p{y} - g\p{y}} \,\diff{y} \,\diff{x} \\
        &= \int_{k/2^n}^{\p{k+1}/2^n} \abs{f\p{y} - g\p{y}} \,\diff{y}.
\end{aligned}
$$

Similarly, by Fubini-Tonelli (everything is non-negative)

$$
\begin{aligned}
    A_{k,n}\p{f\p{x} - g\p{x}}
        &= \int_{k/2^n}^{\p{k+1}/2^n} 2^n \int_{k/2^n}^{\p{k+1}/2^n} \abs{f\p{y} - g\p{y}} \,\diff{y} \,\diff{x} \\
        &= \int_{k/2^n}^{\p{k+1}/2^n} 2^n \int_{k/2^n}^{\p{k+1}/2^n} \abs{f\p{y} - g\p{y}} \,\diff{x} \,\diff{y} \\
        &= \int_{k/2^n}^{\p{k+1}/2^n} \abs{f\p{y} - g\p{y}} \,\diff{y}.
\end{aligned}
$$

Finally, by absolute continuity of $g$ on the compact dyadic square, there exists $\delta > 0$ so that $\abs{x - y} < \delta \implies \abs{g\p{x} - g\p{y}} < \epsilon$. Choose $n$ large enough so that $\frac{1}{2^n} < \delta$ and we get

$$
\begin{aligned}
    \int_{k/2^n}^{\p{k+1}/2^n} A_{k,n}\p{g - g\p{x}} \,\diff{x}
        &= \int_{k/2^n}^{\p{k+1}/2^n} 2^n \int_{k/2^n}^{\p{k+1}/2^n} \abs{g\p{x} - g\p{y}} \,\diff{y} \,\diff{x} \\
        &\leq \int_{k/2^n}^{\p{k+1}/2^n} \epsilon \,\diff{x} \\
        &= \frac{\epsilon}{2^n}.
\end{aligned}
$$

Putting it all together,

$$
\begin{aligned}
    \norm{f_n - f}_{L^1\p{\br{0,1}}}
        &\leq \sum_{k=0}^{2^n-1} \int_{k/2^n}^{\p{k+1}/2^n} A_{k,n}\p{f - g} + A_{k,n}\p{f\p{x} - g\p{x}} + A_{k,n}\p{g - g\p{x}} \,\diff{x} \\
        &\leq \sum_{k=0}^{2^n-1} \p{\int_{k/2^n}^{\p{k+1}/2^n} \abs{f\p{y} - g\p{y}} \,\diff{y} + \int_{k/2^n}^{\p{k+1}/2^n} \abs{f\p{y} - g\p{y}} \,\diff{y} + \frac{\epsilon}{2^n}} \\
        &= 2\norm{f - g}_{L^1\p{\br{0,1}}} + \epsilon \\
        &\leq 3\epsilon.
\end{aligned}
$$

Sending $\epsilon \to 0$, we see $f_n \to f$ in $L^1$, which completes the proof.

</solution>
