---
topics:
    - Hahn-Banach
    - operator theory
    - Banach-Alaoglu
---

<problem>

Let $X$ and $Y$ be Banach spaces. A bounded linear transformation $\func{A}{X}{Y}$ is _compact_ if for every bounded sequence $\set{x_n} \subseteq X$, the sequence $\set{Ax_n}_n$ has a convergent subsequence in $Y$. Suppose $X$ is reflexive ($X^{**} = X$) and $X^*$ is separable. Show that $\func{A}{X}{Y}$ is compact if and only if for every bounded sequence $\set{x_n}_n \subseteq X$, there exists a subsequence $\set{x_{n_j}}_j$ and a vector $\phi \in X$ such that $x_{n_j} = \phi + r_{n_j}$ and $Ar_{n_j} \to 0$ in $Y$.

</problem>

<solution>

"$\impliedby$"

The condition on the subsequence $\set{x_{n_j}}_j$ implies that

$$
Ax_{n_j} = A\phi + Ar_{n_j} \xrightarrow{j\to\infty} A\phi
$$

strongly, i.e., $\set{Ax_{n_j}}_j$ is a convergent subsequence of $\set{Ax_n}$, so $A$ is compact.

"$\implies$"

By applying Banach-Alaoglu to $X^*$, we see that the ball $B^{**}_R = \set{x \in X^{**} \mid \norm{x} \leq R}$ is weakly compact. By reflexivity of $X$, this implies that $B_R = \set{x \in X \mid \norm{x} \leq R}$ is weakly compact.

Given $\set{x_n}_n \subseteq X$, weak compactness implies existence of a subsequence $\set{x_{n_j}}_j$ which converges weakly to some $\phi \in X$. Passing to another subsequence if needed, compactness of $A$ implies that $\set{Ax_{n_j}}_j$ converges strongly to some $y$ in $X$. It remains to show that $y = A\phi$.

Let $f \in Y^*$, and so

$$
\begin{aligned}
    f\p{y}
        &= \lim_{k\to\infty} f\p{Ax_{n_j}}
            && (\text{strong convergence of } Ax_{n_j}) \\
        &= \lim_{k\to\infty} \p{A^\trans f}\p{x_{n_j}} \\
        &= \lim_{k\to\infty} \p{A^\trans f}\p{\phi}
            && (\text{weak convergence of } x_{n_j}) \\
        &= f\p{A\phi}.
\end{aligned}
$$

This implies that $y = A\phi$. Indeed, if this were not the case, then $y - A\phi \neq 0$ and by Hahn-Banach, there exists $f \in Y^*$ such that $f\p{x - y} \neq 0 \implies f\p{x} \neq f\p{y}$, which is impossible. If we set $r_{n_j} = x_{n_j} - \phi$, then $x = \phi + r_{n_j}$ and

$$
Ar_{n_j}
    = Ax_{n_j} - A\phi
    \xrightarrow{k\to\infty} y - A\phi = 0
$$

strongly in $Y$, which completes the proof.

</solution>
