---
topics:
    - Lebesgue differentiation theorem
---

<problem>

Suppose $f \in L^1\p{\R}$ satisfies

$$
\limsup_{h\to0} \int_\R \abs{\frac{f\p{x + h} - f\p{x}}{h}} \,\diff{x} = 0.
$$

</problem>

<solution>

Define

$$
F\p{x} = \int_{-\infty}^x f\p{y} \,\diff{y},
$$

which is well-defined since $f \in L^1\p{\R}$. Observe that

$$
\int_{-\infty}^x f\p{y + h} \,\diff{y}
    = \int_{-\infty}^{x+h} f\p{y} \,\diff{y}
    = F\p{x + h},
$$

so that

$$
\abs{F\p{x + h} - F\p{x}}
    \leq \int_{-\infty}^x \abs{f\p{y + h} - f\p{y}} \,\diff{y}
    \leq \int_\R \abs{f\p{y + h} - f\p{y}} \,\diff{y},
$$

Let $a, b \in \R$ be Lebesgue points. Then for $h > 0$, the calculation above gives

$$
\begin{aligned}
    \frac{1}{2h} \abs{\p{\int_{a-h}^{a+h} f\p{y} \,\diff{y} - \int_{b-h}^{b+h} f\p{y} \,\diff{y}}}
        &= \frac{1}{2h} \abs{\p{F\p{a + h} - F\p{a - h}} - \p{F\p{b + h} - F\p{b - h}}} \\
        &\leq \frac{1}{2h} \p{\abs{F\p{a + h} - F\p{a}} + \abs{F\p{a} - F\p{a - h}} + \abs{F\p{b + h} - F\p{b}} + \abs{F\p{b} - F\p{b - h}}} \\
        &\leq \frac{1}{2h} \cdot 4 \int_\R \abs{f\p{y + h} - f\p{y}} \,\diff{y} \\
        &= 2\int_\R \abs{\frac{f\p{y + h} - f\p{y}}{h}} \,\diff{y}.
\end{aligned}
$$

By the Lebesgue differentiation theorem, we get

$$
\abs{f\p{a} - f\p{b}}
    \leq 2\limsup_{h\to0} \int_\R \abs{\frac{f\p{y + h} - f\p{y}}{h}} \,\diff{y}
    = 0,
$$

by assumption, i.e., $f\p{a} = f\p{b}$. Thus, because almost every $x \in \R$ is a Lebesgue point, we see that $f$ must be a constant. Since $f \in L^1\p{\R}$, it follows that $f = 0$, which was what we wanted to show.

</solution>
