---
topics:
    - Lp spaces
---

<problem>

Suppose $f \in L^1\p{\R}$ satisfies

$$
\limsup_{\epsilon\to0} \int_\R \int_\R \frac{\abs{f\p{x}}\abs{f\p{y}}}{\abs{x - y}^2 + \epsilon^2} \,\diff{x} \,\diff{y} < \infty.
$$

Show that $f = 0$ almost everywhere.

</problem>

<solution>

First, assume that $f = \chi_E$. Assume otherwise, and that $\chi_E \neq 0$ almost everywhere, i.e., $m\p{E} > 0$. Then

$$
\begin{aligned}
    \int_\R \int_\R \frac{\abs{f\p{x}}\abs{f\p{y}}}{\abs{x - y}^2 + \epsilon^2} \,\diff{x} \,\diff{y}
        &= \int_\R \int_\R \frac{\chi_E\p{x + y} \chi_E\p{y}}{\abs{x}^2 + \epsilon^2} \,\diff{x} \,\diff{y}
            && \p{x \mapsto x + y} \\
        &= \int_\R \frac{1}{\abs{x}^2 + \epsilon^2} \int_\R \chi_E\p{x + y} \chi_E\p{y} \,\diff{y} \,\diff{x}.
\end{aligned}
$$

Since translation is continuous in $L^1\p{\R}$, we see that

$$
\lim_{x\to0} \int_\R \chi_E\p{x + y} \chi_E\p{y} \,\diff{y}
    = \lim_{x\to0} \int_E \chi_E\p{x + y} \,\diff{y}
    = \int_E \chi_E\p{y} \,\diff{y}
    = m\p{E}
    > 0.
$$

Thus, there exists $\delta > 0$ so that if $\abs{x} < \delta$, then $\int_\R \chi_E\p{x + y}\chi_E\p{y} \,\diff{y} \geq \frac{m\p{E}}{2}$. Hence, if $\epsilon < 1$,

$$
\begin{aligned}
    \int_\R \frac{1}{\abs{x}^2 + \epsilon^2} \int_\R \chi_E\p{x + y} \chi_E\p{y} \,\diff{y} \,\diff{x}
        &\geq \frac{m\p{E}}{2} \int_{B\p{0,\delta}} \frac{1}{\abs{x}^2 + \epsilon^2} \,\diff{x} \\
        &= m\p{E} \int_0^\delta \frac{1}{x^2 + \epsilon} \,\diff{x} \\
        &= \frac{m\p{E}}{\epsilon} \arctan\p{\frac{\delta}{\epsilon}} \\
        &\geq \frac{m\p{E}}{\epsilon} \arctan\,\p{\delta}
            \xrightarrow{\epsilon\to0} \infty.
\end{aligned}
$$

Hence, if $f = \chi_E$, then it must be that $m\p{E} = 0$. For the general case, suppose $f \neq 0$, and so there exist $a > 0$ and $E \subseteq \R$ measurable such that $\abs{f} \geq a\chi_E$. Then

$$
\int_\R \int_\R \frac{\abs{f\p{x}}\abs{f\p{y}}}{\abs{x - y}^2 + \epsilon^2} \,\diff{x} \,\diff{y}
    \geq a^2 \int_\R \int_\R \frac{\chi_E\p{x} \chi_E\p{y}}{\abs{x - y}^2 + \epsilon^2} \,\diff{x} \,\diff{y}
    \xrightarrow{\epsilon\to0} \infty.
$$

Thus, $f = 0$ almost everywhere, which was what we wanted to show.

</solution>
