---
topics:
    - residue theorem
    - calculation
---

<problem>

Determine

$$
\int_0^\infty \frac{x^{a-1}}{x + z} \,\diff{x},
$$

for $0 < a < 1$ and $\Re{z} > 0$. Justify all manipulations.

</problem>

<solution>

Set $f\p{w} = \frac{w^{a-1}}{w + z}$ and for $0 < \epsilon < \abs{z} < R$ and $\alpha \in \p{0, \pi}$, let $\gamma_{\epsilon,R,\alpha}$ be the boundary of

$$
\set{z \in \C \mid \epsilon < \abs{z} < R \text{ and } \alpha < \Arg{z} < 2\pi - \alpha},
$$

where we take the standard branch of $\Arg{z}$ with branch cut on the positive real axis. On the arc $C_R$ of radius $R$, we have

$$
\begin{aligned}
    \abs{\int_{C_R} f\p{w} \,\diff{w}}
        &= \abs{\int_\alpha^{2\pi-\alpha} \frac{R^{a-1}e^{i\p{a-1}\theta}}{Re^{i\p{a-1}\theta} + z} iRe^{i\theta} \,\diff\theta} \\
        &\leq \int_0^{2\pi} \frac{R^a}{R - \abs{z}} \,\diff\theta \\
        &= \frac{2\pi R^a}{R - \abs{z}}
            \xrightarrow{R\to\infty} 0,
\end{aligned}
$$

since $a < 1$, so this contribution tends to $0$ uniformly in $\alpha$. Similarly, on the arc $C_\epsilon$ of radius $\epsilon$,

$$
\abs{\int_{C_\epsilon} f\p{w} \,\diff{w}}
    \leq \frac{2\pi \epsilon^a}{\abs{z} - \epsilon}
    \xrightarrow{\epsilon\to0},
$$

since $a > 0$, uniformly in $\alpha$ as well. Finally, in the limit as $\alpha \to 0$, the contribution from the segment $\br{\epsilon e^{i\p{2\pi-\alpha}}, Re^{i\p{2\pi-\alpha}}}$ becomes

$$
\int_\epsilon^R \frac{t^{a-1} e^{i\p{a-1}\p{2\pi-\alpha}}}{te^{i\p{2\pi-\alpha}} + z} e^{i\p{2\pi-\alpha}} \,\diff{t}
    \xrightarrow{\alpha\to0} e^{2\pi i\p{a-1}} \int_\epsilon^R \frac{t^{a-1}}{t + z} \,\diff{t}.
$$

Indeed, the integrand is bounded and $\br{\epsilon, R}$ is compact, so we may apply dominated convergence to send $\alpha \to 0$. $f$ only has one residue at $w = -z$, which is

$$
\Res{f}{-z}
    = \p{-z}^{a-1},
$$

which is well-defined since $\Re{z} > 0$, so $-z$ avoids the positive real axis. Thus, by the residue theorem and sending $\alpha \to 0$, $\epsilon \to 0$, and $R \to \infty$, we get

$$
\p{1 + e^{2\pi i\p{a-1}}} \int_0^\infty \frac{x^{a-1}}{x + z} \,\diff{x}
    = 2\pi i \p{-z}^{a-1}
\implies \int_0^\infty \frac{x^{a-1}}{x + z} \,\diff{x} = \frac{2\pi i \p{-z}^{a-1}}{1 + e^{2\pi i\p{a-1}}}.
$$

</solution>
