---
topics:
    - density argument
---

<problem>

Given $\func{f}{\br{0,1}}{\R}$ belonging to $L^1\p{\diff{x}}$ and $n \in \set{1, 2, 3, \ldots}$ define

$$
f_n\p{x} = n \int_{k/n}^{\p{k+1}/n} f\p{y} \,\diff{y}
\quad\text{for } x \in \pco{\frac{k}{n}, \frac{k+1}{n}}
\quad\text{and}\quad k = 0, \ldots, n-1.
$$

Prove $f_n \to f$ in $L^1$.

</problem>

<solution>

Notice that

$$
n \int_{k/n}^{\p{k+1}/n} \,\diff{y}
    = n \cdot \frac{1}{n}
    = 1
$$

for any $k = 0, \ldots, n-1$.

Let $\epsilon > 0$. Since $C\p{\br{0, 1}}$ is dense in $L^1\p{\br{0, 1}}$, there exists a continuous $g$ such that $\norm{f - g}_{L^1} < \epsilon$. Since $\br{0, 1}$ is compact, $g$ is uniformly continuous, so there exists $\delta > 0$ so that $\abs{x - y} < \delta \implies \abs{g\p{x} - g\p{y}} < \epsilon$.

$$
\begin{aligned}
    \norm{f_n - f}_{L^1}
        &= \int \abs{f_n\p{x} - f\p{x}} \,\diff{x} \\
        &= \sum_{k=0}^{n-1} \int_{k/n}^{\p{k+1}/n} n\abs{\int_{k/n}^{\p{k+1}/n} f\p{y} - f\p{x} \,\diff{y}} \,\diff{x} \\
        &\leq \sum_{k=0}^{n-1} \int_{k/n}^{\p{k+1}/n} n\int_{k/n}^{\p{k+1}/n} \abs{f\p{y} - f\p{x}} \,\diff{y} \,\diff{x} \\
        &\leq \sum_{k=0}^{n-1} \int_{k/n}^{\p{k+1}/n} n\int_{k/n}^{\p{k+1}/n} \abs{f\p{y} - g\p{y}} + \abs{g\p{y} - g\p{x}} + \abs{g\p{x} - f\p{x}} \,\diff{y} \,\diff{x}.
\end{aligned}
$$

We will look at each term separately: In the following, everything is non-negative, so by Fubini-Tonelli,

$$
\begin{aligned}
    \sum_{k=0}^{n-1} \int_{k/n}^{\p{k+1}/n} n\int_{k/n}^{\p{k+1}/n} \abs{f\p{y} - g\p{y}} \,\diff{y} \,\diff{x}
        &= \sum_{k=0}^{n-1} \int_{k/n}^{\p{k+1}/n} n\int_{k/n}^{\p{k+1}/n} \abs{f\p{y} - g\p{y}} \,\diff{x} \,\diff{y} \\
        &= \sum_{k=0}^{n-1} \int_{k/n}^{\p{k+1}/n} \abs{f\p{y} - g\p{y}} \,\diff{y} \\
        &= \norm{f - g}_{L^1} \\
        &\leq \epsilon.
\end{aligned}
$$

Similarly,

$$
\begin{aligned}
    \sum_{k=0}^{n-1} \int_{k/n}^{\p{k+1}/n} n\int_{k/n}^{\p{k+1}/n} \abs{f\p{x} - g\p{x}} \,\diff{y} \,\diff{x}
        &= \sum_{k=0}^{n-1} \int_{k/n}^{\p{k+1}/n} \abs{f\p{x} - g\p{x}} \,\diff{x} \\
        &= \norm{f - g}_{L^1} \\
        &\leq \epsilon
\end{aligned}
$$

Finally, if $n$ is large enough, then

$$
\begin{aligned}
    \sum_{k=0}^{n-1} \int_{k/n}^{\p{k+1}/n} n\int_{k/n}^{\p{k+1}/n} \abs{g\p{y} - g\p{x}} \,\diff{y} \,\diff{x}
        &\leq \sum_{k=0}^{n-1} \int_{k/n}^{\p{k+1}/n} n\int_{k/n}^{\p{k+1}/n} \epsilon \,\diff{y} \,\diff{x} \\
        &= \epsilon.
\end{aligned}
$$

Overall, we get $\norm{f_n - f}_{L^1} \leq 3\epsilon$. Sending $\epsilon \to 0$, we get the claim.

</solution>
