---
topics:
    - residue theorem
    - Riemann Zeta function
---

<problem>

Consider the function defined for $s \in \p{1, \infty}$ by

$$
f\p{s} = \int_0^\infty \frac{x^{s-1}}{e^x - 1} \,\diff{x}.
$$

Show that $f$ has an analytic continuation to $\set{s \in \C \mid \Re{s} > 0, s \neq 1}$ with a simple pole at $s = 1$. Compute the residue at $s = 1$.

</problem>

<solution>

We have $a^{s-1} = e^{\p{s-1}\log{a}}$ for $a > 0$. We split $f$ up into

$$
f\p{s}
    = \int_0^1 \frac{x^{s-1}}{e^x - 1} \,\diff{x} + \int_1^\infty \frac{x^{s-1}}{e^x - 1} \,\diff{x}
    \eqqcolon I_1\p{s} + I_2\p{s}.
$$

Notice that

$$
I_2\p{s}
    = \p{\int_1^\infty \sum_{n=0}^\infty \frac{\p{\log{x}}^n}{e^x - 1} \,\diff{x}}\p{s - 1}^n
    = \sum_{n=0}^\infty \p{\int_1^\infty \frac{\p{\log{x}}^n}{e^x - 1} \,\diff{x}}\p{s - 1}^n,
$$

by the monotone convergence theorem, since each term in the sum is non-negative. Since $I_2$ has no singularities, this series expansion is valid on the entire complex plane, so $I_2$ is entire.

It remains to show that $I_1$ is analytic on the right-half plane except at $s = 1$. Observe that

$$
g\p{s}
    \coloneqq I_1\p{s} - \frac{1}{s - 1}
    = \int_0^1 x^{s-1}\p{\frac{1}{e^x - 1} - \frac{1}{x}} \,\diff{x}.
$$

Then by L'HÃ´pital's,

$$
\lim_{x\to0}\,\p{\frac{1}{e^x - 1} - \frac{1}{x}}
    = \lim_{x\to0} \frac{x - e^x + 1}{x\p{e^x - 1}}
    = \lim_{x\to0} \frac{1 - e^x}{e^x - 1 + xe^x}
    = \lim_{x\to0} \frac{-e^x}{e^x + e^x + xe^x}
    = -\frac{1}{2},
$$

so the integrand is continuous on $\br{0, 1}$, and so $g$ is well-defined. Hence, the integral converges whenever $s - 1 > 1 \implies s > 0$ and so $g$ is analytic on $\Re{s} > 0$ by differentiating under the integral sign. We then have the representation

$$
I_1\p{s} = g\p{s} + \frac{1}{s - 1},
$$

so $I_1\p{s}$ is analytic on $\Re{s} > 0$ except at $s = 1$, and it has a simple pole at $s = 1$, and so $f\p{s}$ satisfies the same properties. To calculate the residue at $s = 1$,

$$
\lim_{s\to1}\,\p{s - 1}f\p{s}
    = \lim_{s\to1}\, \p{\p{s - 1}g\p{s} + 1 + \p{s - 1}I_2\p{s}}
    = 1,
$$

and this completes the proof.

</solution>
