---
topics:
    - Hadamard factorization
---

<problem>

Show that

$$
\sin{z} - z\cos{z}
    = \frac{z^3}{3} \prod_{n=1}^\infty \p{1 - \frac{z^2}{\lambda_n^2}},
\quad z \in \C,
$$

where $\set{\lambda_n}_n$ is a sequence in $\C$, $\lambda_n \neq 0$ for all $n$, such that

$$
\sum_{n=1}^\infty \frac{1}{\abs{\lambda_n}^2} < \infty.
$$

</problem>

<solution>

Let $f\p{z} = \sin{z} - z\cos{z}$. Notice that $f\p{-z} = -\sin{z} + z\cos{z} = -f\p{z}$. Thus, if $\lambda$ is a root of $f$, then so is $-\lambda$. Let $\set{-\lambda_n, \lambda_n}_n$ be the non-zero zeroes of $f$ counted with multiplicity. At the origin, we have

$$
\begin{aligned}
    f\p{0}
        &= 0 \\
    f'\p{z} = z\sin{z}
    \implies
    f'\p{0}
        &= 0 \\
    f''\p{z} = \sin{z} + z\cos{z}
    \implies
    f''\p{0}
        &= 0 \\
    f'''\p{z} = 2\cos{z} - z\sin{z}
    \implies
    f'''\p{0}
        &= 2,
\end{aligned}
$$

so $f$ has a zero of order $3$ at the origin. $f$ is also entire of first order since $z, \sin{z}, \cos{z}$ all are, so by Hadamard factorization,

$$
f\p{z} = e^{az+b} z^3 \prod_{n=1}^\infty \p{1 - \frac{z^2}{\lambda_n^2}}
$$

with

$$
\sum_{n=1}^\infty \frac{1}{\abs{\lambda_n}^2} < \infty.
$$

To complete the proof, we need to calculate $a, b \in \C$. Notice that if $a_3$ is the coefficient of $z^3$ in the Taylor series of $f$, then

$$
e^b
    = \lim_{z\to0} \frac{f\p{z}}{z^3}
    = a_3
    = \frac{f'''\p{0}}{3!}
    = \frac{1}{3}.
$$

For $a$, notice that

$$
-1
    = \frac{f\p{z}}{f\p{-z}}
    = -e^{-az}
\implies a = 0,
$$

and so

$$
\sin{z} - z\cos{z}
    = \frac{z^3}{3} \prod_{n=1}^\infty \p{1 - \frac{z^2}{\lambda_n^2}}.
$$

</solution>
