---
topics:
    - analytic continuation
---

<problem>

Define

$$
f\p{z}
    = \int_0^1 \frac{t^z}{e^t - 1} \,\diff{t},
\quad z \in \C,\ \Re{z} > 0.
$$

Show that $f$ is an analytic function in $\set{z \in \C \st \Re{z} > 0}$ and that it admits a meromorphic continuation $\hat{f}$ to the region $\set{z \in \C \st \Re{z} > -1}$. Compute the residue of $\hat{f}$ at $z = 0$.

</problem>

<solution>

Notice that because $1 + t \leq e^t$, we have $t \leq e^t - 1$, so

$$
\abs{\frac{t^z}{e^t - 1}}
    \leq \frac{t^{\Re{z}}}{t}
    = t^{\Re{z}-1} \in L^1\p{\br{0,1}},
$$

since $\Re{z} - 1 > -1$. Thus, $f$ is well-defined, and we may also apply dominated convergence to see that $f$ is continuous. Hence, given any closed $\gamma \subseteq \set{\Re{z} > 0}$, we have $a = \inf_{z \in \gamma} \Re{z} > 0$, and so

$$
\int_\gamma \int_0^1 \abs{\frac{t^z}{e^t - 1}} \,\diff{t} \,\diff{z}
    \leq \abs{\gamma} \int_0^1 t^{a - 1} \,\diff{t}
    < \infty.
$$

Thus, we may apply Fubini's theorem to get

$$
\int_\gamma f\p{z} \,\diff{z}
    = \int_0^1 \frac{1}{e^t - 1} \int_\gamma t^z \,\diff{z} \,\diff{t}
    = 0,
$$

since the inner integral is $0$ for every $t \in \br{0, 1}$. Thus, by Morera's theorem, $f$ is holomorphic on $\set{\Re{z} > 0}$. For the second claim, we integrate by parts to see

$$
\begin{aligned}
    f\p{z}
        &= \int_0^1 t^{z-1} \cdot \frac{t}{e^t - 1} \,\diff{t} \\
        &= \left. \frac{t^z}{z\p{e^t - 1}} \right\rvert_0^1 + \frac{1}{z} \int_0^1 t^z \cdot \frac{e^t\p{t - 1} + 1}{\p{e^t - 1}^2} \,\diff{t} \\
        &= \frac{1}{z\p{e - 1}} + \frac{1}{z} \int_0^1 \frac{t^z\br{e^t\p{t - 1} + 1}}{\p{e^t - 1}^2} \,\diff{t}.
\end{aligned}
$$

and the integral term is holomorphic on $\set{\Re{z} > -1}$ by the same argument as before. Indeed, notice

$$
e^t\p{t - 1} + 1
    \leq \p{1 + t}\p{t - 1} + 1
    = t^2.
$$

Thus,

$$
\abs{\frac{t^z\br{e^t\p{t - 1} + 1}}{\p{e^t - 1}^2}}
    \leq \frac{t^{\Re{z}} t^2}{t^2}
    = t^{\Re{z}}
$$

which is integrable on $\Re{z} > -1$. Finally, the residue at $z = 0$ is given by

$$
\begin{aligned}
    \Res{f}{0}
        &= \frac{1}{e - 1} + \int_0^1 \frac{e^t\p{t - 1} + 1}{\p{e^t - 1}^2} \,\diff{t} \\
        &= \frac{1}{e - 1} - \left. \frac{t}{e^t - 1} \right\rvert_0^1 \\
        &= 1.
\end{aligned}
$$

</solution>
