---
topics:
    - entire functions
---

<problem>

Consider a map $\func{F}{\C \times \C}{\C}$ with the following properties:

1. For each fixed $z \in \C$ the map $w \mapsto F\p{z, w}$ is injective.
2. For each fixed $w \in \C$ the map $z \mapsto F\p{z, w}$ is holomorphic.
3. $F\p{0, w} = w$ for $w \in \C$.

Show that then

$$
F\p{z, w} = a\p{z}w + b\p{z}
$$

for $z, w \in \C$, where $a$ and $b$ are entire functions with $a\p{0} = 1$, $b\p{0} = 0$, and $a\p{z} \neq 0$ for $z \in \C$.

_Hint:_ Consider $\frac{F\p{z, w} - F\p{z, 0}}{F\p{z, 1} - F\p{z, 0}}$.

</problem>

<solution>

Let $G\p{z, w} = \frac{F\p{z, w} - F\p{z, 0}}{F\p{z, 1} - F\p{z, 0}}$. By injectivity, $F\p{z, 1} - F\p{z, 0} \neq 0$ for any $z \in \C$, so $z \mapsto G\p{z, w}$ is entire.

Notice that $G\p{z, 0} = 0$ and $G\p{z, 1} = 1$. If $w \neq 1, 2$, then by injectivity, $F\p{z, w} \neq F\p{z, 0}$ and $F\p{z, w} \neq F\p{z, 1}$, so $G\p{z, w}$ misses $0$ and $1$. By Picard's little theorem, $z \mapsto G\p{z, w}$ is constant. In all cases, $z \mapsto G\p{z, w}$ is constant, so

$$
G\p{z, w}
    = G\p{0, w}
    = \frac{F\p{0, w} - F\p{0, 0}}{F\p{0, 1} - F\p{0, 0}}
    = w.
$$

Thus,

$$
w = \frac{F\p{z, w} - F\p{z, 0}}{F\p{z, 1} - F\p{z, 0}}
\implies
F\p{z, w} = \p{F\p{z, 1} - F\p{z, 0}}w + F\p{z, 0}.
$$

If we set $a\p{z} = F\p{z, 1} - F\p{z, 0}$ and $b\p{z} = F\p{z, 0}$, then $a\p{0} = 0$, $b\p{0} = 0$, and by injectivity, $a\p{z} \neq 0$, which completes the proof.

</solution>
