---
topics:
    - calculation
---

<problem>

Consider the meromorphic function $g\p{z} = -\pi z\cot\p{\pi z}$ on the entire plane $\C$.

1. Find all poles of $g$ and determine the residue of $g$ at each pole.
2. In the Taylor series representation $\sum_{k=0}^\infty a_kz^k$ of $g\p{z}$ about $z = 0$, show that for each $k \geq 1$,

    $$
    a_{2k} = \sum_{n\geq1} \frac{2}{n^{2k}}.
    $$

</problem>

<solution>

1. Since $\cot\p{\pi z} = \frac{\cos\p{\pi z}}{\sin\p{\pi z}}$, it follows that $\cot{\pi z}$ has simple poles at every integer. Thus, $g$ has a simple pole at every non-zero integer, and these have residue given by

    $$
    \begin{aligned}
        \Res{g}{k}
            &= \lim_{z \to k} \,\p{z - k}g\p{z} \\
            &= \p{\lim_{z \to k} -\pi z\cos\p{\pi z}} \p{\lim_{x \to k} \frac{x - k}{\sin\p{\pi x}}} \\
            &= -\pi k\cos\p{\pi k} \p{\lim_{x \to k} \frac{1}{\pi\cos\p{\pi x}}} \\
            &= -k.
    \end{aligned}
    $$

2. Recall that $\pi\cot\p{\pi z}$ has the expansion

    $$
    \pi \cot\p{\pi z}
        = \frac{1}{z} + \sum_{n=1}^\infty \frac{2z}{z^2 - n^2}
    \implies
    g\p{z}
        = -1 - \sum_{n=1}^\infty \frac{2z^2}{z^2 - n^2}.
    $$

    Let $f\p{z} = -1 - \sum_{n=1}^\infty \frac{2z}{z - n^2}$ so that $f\p{z^2} = g\p{z}$, i.e., the $k$-th coefficient in the Maclaurin series expansion of $f$ corresponds to the $2k$-th coefficient of $g$. Observe that if $k \geq 1$,

    $$
    \begin{aligned}
        \p{\deriv{^k}{x^k} f\p{z}}\p{0}
            &= -\sum_{n=1}^\infty \p{\sum_{m=0}^k \binom{k}{m} \p{\deriv{^m}{x^m} z}\p{0} \p{\deriv{^{k-m}}{x^{k-m}} \frac{2}{z - n^2}}\p{0}} \\
            &= -\sum_{n=1}^\infty \binom{k}{1} \p{\deriv{^{k-1}}{x^{k-1}} \frac{2}{z - n^2}}\p{0} \\
            &= -\sum_{n=1}^\infty \frac{2k\p{-1}^{k-1}\p{k-1}!}{\p{-n^2}^k} \\
            &= \sum_{n=1}^\infty \frac{2 \cdot k!}{n^{2k}}.
    \end{aligned}
    $$

    Thus, if $b_k$ is the $k$-th coefficient of the Maclaurin series of $f$, then

    $$
    a_{2k}
        = b_k
        = \frac{1}{k!} \sum_{n=1}^\infty \frac{2 \cdot k!}{n^{2k}}
        = \sum_{n=1}^\infty \frac{2}{n^{2k}}.
    $$

</solution>
