---
topics:
    - residue theorem
    - calculation
---

<problem>

Let $f\p{z} = -\pi z\cot\p{\pi z}$ as a meromorphic function on the whole of $\C$.

1. Locate all poles of $f$ and determine their residues.
2. Show that for each $n \geq 1$ the coefficient of $z^{2n}$ in the Taylor expansion of $f\p{z}$ about $z = 0$ coincides with

    $$
    a_n = \sum_{k=1}^\infty \frac{2}{k^{2n}}.
    $$

</problem>

<solution>

1. The poles of $f$ are precisely the poles of $\frac{z}{\sin{\pi z}}$ since $\cos{\pi z}$ is entire. Since $\sin{\pi z}$ has a simple pole at $0$, it follows that $\frac{z}{\sin{\pi z}}$ is analytic near the origin, so the poles of $f$ are at $\Z \setminus \set{0}$. Given $k \in \Z \setminus \set{0}$, $\sin{\pi z}$ has a simple zero at $k$, so we may take the following limit from the real direction and apply L'HÃ´pital's:

    $$
    \begin{aligned}
       \Res{f}{k}
           &= \lim_{z \to k} \p{z - k}f\p{z} \\
           &= -\pi \lim_{x \to k} \frac{x\p{x - k}}{\sin{\pi x}} \\
           &= -\pi \lim_{x \to k} \frac{x + x - k}{\pi\cos{\pi x}} \\
           &= -\frac{k}{\cos{\pi k}} \\
           &= \p{-1}^{k+1} k.
    \end{aligned}
    $$

2. We have the representation

    $$
    \pi \cot{\pi z} = \frac{1}{z} + \sum_{k=1}^\infty \frac{2z}{z^2 - k^2}
    \implies f\p{z} = -1 - \sum_{k=1}^\infty \frac{2z^2}{z^2 - k^2}.
    $$

    Set $g\p{z} = \sum_{k=1}^\infty \frac{2}{z^2 - k^2}$ so that $f\p{z} = -1 - z^2g\p{z}$. Then

    $$
    \begin{aligned}
       f^{\p{2n}}\p{0}
           &= -\sum_{j=0}^{2n} \binom{2n}{j} \p{\frac{\diff^j}{\diff{z}^j} z^2}\p{0} g^{\p{2n-j}}\p{0} \\
           &= -2\frac{\p{2n}!}{2!\p{2n - 2}!} g^{\p{2n-2}}\p{0} \\
           &= -\p{2n}\p{2n - 1} g^{\p{2n-2}}\p{0} \\
    \end{aligned}
    $$

    Since $g$ is a Laurent series, it converges uniformly on compact sets, so we may differentiate term-by-term. Notice that

    $$
    \frac{2z^2}{z^2 - k^2}
        = 2 + \frac{2k^2}{z^2 - k^2}
        = 2 + k\p{\frac{1}{z - k} - \frac{1}{z + k}}
    $$

    and so

    $$
    \begin{aligned}
        g^{\p{2n-2}}\p{z}
            &= \sum_{k=1}^\infty k\p{\p{-1}^{2n-2}\frac{\p{2n - 2}!}{\p{z - k}^{2n-1}} - \p{-1}^{2n-2}\frac{\p{2n - 2}!}{\p{z + k}^{2n-1}}} \\
            &= \sum_{k=1}^\infty k\p{\frac{\p{2n - 2}!}{\p{z - k}^{2n-1}} - \frac{\p{2n - 2}!}{\p{z + k}^{2n-1}}} \\
        g^{\p{2n-2}}\p{0}
            &= \sum_{k=1}^\infty k\p{\frac{\p{2n - 2}!}{\p{-k}^{2n-1}} - \frac{\p{2n - 2}!}{k^{2n-1}}} \\
            &= -2 \sum_{k=1}^\infty \frac{\p{2n - 2}!}{k^{2n}}.
    \end{aligned}
    $$

    Hence,

    $$
    f^{\p{2n}}\p{0} = 2\sum_{k=1}^\infty \frac{n!}{k^{2n}}
    \implies \frac{f^{\p{2n}}\p{0}}{\p{2n}!} = \sum_{k=1}^\infty \frac{2}{k^{2n}}.
    $$

</solution>
