---
topics:
    - residue theorem
    - calculation
---

<problem>

Determine

$$
\int_{-\infty}^\infty \frac{\diff{y}}{\p{1 + y^2}\p{1 + \p{x-y}^2}}
$$

for all $x \in \R$. Justify all manipulations.

</problem>

<solution>

Let $f\p{z} = \frac{1}{\p{1 + z^2}\p{1 + \p{x-z}^2}}$, which has poles at $\pm i$ and

$$
1 + \p{x - z}^2 = 0
\iff x \pm i.
$$

For $0 < R < \abs{x + i}$, let $\gamma_R$ be the semicircle with $\br{-R, R}$ and arc $\set{Re^{i\theta} \mid 0 \leq \theta \leq \pi}$. Then the only poles of $f$ in the interior of $\gamma_R$ are $i$ and $x + i$. The residues of $f$ there are

$$
\begin{aligned}
    \Res{f}{i}
        &= \lim_{z \to i} \p{z - i} f\p{z} \\
        &= \lim_{z \to i} \frac{1}{\p{i + z}\p{1 + \p{x - z}^2}} \\
        &= \frac{1}{2i\p{1 + \p{x - i}^2}}
\end{aligned}
$$

and

$$
\begin{aligned}
    \Res{f}{x + i}
        &= \lim_{z \to x+i} \p{z - \p{x+i}}f\p{z} \\
        &= \lim_{z \to x+i} \frac{1}{\p{1 + z^2}\p{\p{z - x} + i}} \\
        &= \frac{1}{2i\p{1 + \p{x+i}^2}}.
\end{aligned}
$$

As for the integral, on the arc $C_R$, we get

$$
\begin{aligned}
    \abs{\int_{C_R} f\p{z} \,\diff{z}}
        &= \abs{\int_0^\pi \frac{iRe^{i\theta}}{\p{1 + R^2e^{i2\theta}}\p{1 + \p{x - Re^{i\theta}}^2}} \,\diff\theta} \\
        &\leq \int_0^\pi \frac{R}{\p{R^2 - 1}\p{R^2 - \p{1 + x}}^2} \,\diff\theta \\
        &= \frac{\pi R}{\p{R^2 - 1}\p{R^2 - \p{1 + x}}^2}
\end{aligned}
$$

which tends to $0$ as $R \to \infty$. Thus, by the residue theorem, sending $R \to \infty$ yields

$$
\begin{aligned}
    \int_{-\infty}^\infty \frac{\diff{y}}{\p{1 + y^2}\p{1 + \p{x-y}^2}}
        &= 2\pi i \p{\frac{1}{2i\p{1 + \p{x - i}^2}} + \frac{1}{2i\p{1 + \p{x+i}^2}}} \\
        &= \pi\p{\frac{1 + \p{x + i}^2 + 1 + \p{x - i}^2}{\p{1 + \p{x - i}^2}\p{1 + \p{x + i}^2}}} \\
        &= \pi\p{\frac{2 + 2x^2 - 2}{1 + \p{x + i}^2 + \p{x - i}^2 + \p{x - i}^2\p{x + i}^2}} \\
        &= \pi\p{\frac{2x^2}{1 + 2x^2 - 2 + x^4 + 2x^2 + 1}} \\
        &= \frac{2\pi}{x^2 + 4}.
\end{aligned}
$$

</solution>
