---
topics:
    - residue theorem
    - calculation
---

<problem>

Evaluate the improper Riemann integral

$$
\int_0^\infty \frac{x^2 - 1}{x^2 + 1} \frac{\sin{x}}{x} \,\diff{x}.
$$

Justify all manipulations.

</problem>

<solution>

Let $f\p{z} = \frac{z^2 - 1}{z^2 + 1} \frac{e^{iz}}{z}$. For $0 < \epsilon < R$, let $\gamma_{\epsilon,R}$ be the contour

$$
\gamma_{\epsilon,R}
    = \br{\epsilon, R} \cup \set{Re^{i\theta} \st 0 \leq \theta \leq \pi} \cup \br{-R, -\epsilon} \cup \set{\epsilon e^{i\theta} \st 0 \leq \theta \leq \pi}
$$

oriented counter-clockwise. On the large semi-circle $C_R$, we have

$$
\begin{aligned}
    \abs{\int_{C_R} f\p{z} \,\diff{z}}
        &\leq \int_0^\pi \frac{R^2 + 1}{R^2 - 1} e^{-R\sin\theta} \,\diff\theta \\
        &= \frac{2\p{R^2 + 1}}{R^2 - 1} \int_0^{\pi/2} e^{-R\sin\theta} \,\diff\theta \\
        &\leq \frac{2\p{R^2 + 1}}{R^2 - 1} \int_0^{\pi/2} e^{-2R\theta/\pi} \,\diff\theta \\
        &= \frac{\pi\p{R^2 + 1}}{R\p{R^2 - 1}} \p{1 - e^{-R}}
            \xrightarrow{R\to\infty} 0.
\end{aligned}
$$

On $C_\epsilon$, we get a half residue in the limit: Notice that $f\p{z} + \frac{1}{z}$ is holomorphic near $z = 0$ since $f$ has residue $-1$ there, so it is bounded near $z = 0$ by some $M > 0$. Hence,

$$
\begin{gathered}
    \abs{\int_{C_\epsilon} f\p{z} + \frac{1}{z} \,\diff{z}}
        \leq M\abs{C_\epsilon} \xrightarrow{\epsilon\to0} 0 \\
    \implies
    \lim_{\epsilon\to0} \int_{C_\epsilon} f\p{z} \,\diff{z}
        = \pi i.
\end{gathered}
$$

Finally, our $\gamma_{\epsilon,R}$ contains a pole at $z = i$, which gives the residue

$$
\Res{f}{i}
    = \lim_{z\to i} \,\p{z - i}f\p{z}
    = \lim_{z\to i} \frac{z^2 - 1}{z + i} \frac{e^{iz}}{z}
    = e^{-1}.
$$

Thus, by the residue theorem, sending $\epsilon \to 0$ and $R \to \infty$, we get

$$
\int_{-\infty}^\infty \frac{x^2 - 1}{x^2 + 1} \frac{e^{ix}}{x} \,\diff{x}
    = 2\pi i e^{-1} - \pi i.
$$

Taking imaginary parts and noting that the integrand is even, we have

$$
\int_0^\infty \frac{x^2 - 1}{x^2 + 1} \frac{\sin{x}}{x} \,\diff{x}
    = \frac{\pi}{e} - \frac{\pi}{2}.
$$

</solution>
